aneris/examples/snapshot_isolation/specs/specs_variants/resources_local_pointers.v
@@ -5,12 +5,14 @@ From aneris.aneris_lang Require Export resources.
 From aneris.examples.reliable_communication.prelude
      Require Import list_minus.
 From aneris.examples.snapshot_isolation.specs
-     Require Export user_params time events.
+     Require Export user_params time.
+From aneris.examples.snapshot_isolation.specs.specs_variants
+     Require Export events_local_pointers.
 
 Section Resources.
 
-  Reserved Notation "k ↦ₖ eo" (at level 20).
-  Reserved Notation "k ↦{ c } vo" (at level 20).
+  Reserved Notation "k ↦ₖ e" (at level 20).
+  Reserved Notation "k ↦ₜ c" (at level 20).
 
   Inductive local_state `{!KVS_time}: Type :=
    | CanStart
@@ -25,22 +27,16 @@ Section Resources.
 
     (** Logical global points-to connective *)
     OwnMemKey : Key → option write_event → iProp Σ
-    where "k ↦ₖ we" := (OwnMemKey k we);
+    where "k ↦ₖ v" := (OwnMemKey k v);
 
    (** Logical Local points-to connective *)
-    OwnLocalKey : Key → val → option val → iProp Σ
-    where "k ↦{ c } vo" := (OwnLocalKey k c vo);
+    OwnLocalKey : Key → cache_event → iProp Σ
+    where "k ↦ₜ c" := (OwnLocalKey k c);
 
-   (** Logical points-to connective *)
+    (** Logical points-to connective *)
     ConnectionState : val → local_state → iProp Σ;
 
     KVS_si : message → iProp Σ;
-
-   (** Cache Key Status *)
-    KeyUpdStatus : val → Key → bool → iProp Σ;
-
-    KeyUpdStatus_exclusive c k b b' :
-      KeyUpdStatus c k b ⊢ KeyUpdStatus c k b' -∗ False;
 
     (** Properties of points-to connective *)
     OwnMemKey_timeless k v :> Timeless (k ↦ₖ v);
@@ -53,9 +49,9 @@ Section Resources.
       k ↦ₖ Some we ∗ ⌜we_key we = k⌝;
 
 (** Properties of local points-to connective *)
-    OwnLocalKey_timeless k v c:> Timeless (k ↦{c} v);
-    OwnLocalKey_exclusive k c v v' :
-      k ↦{c} v ⊢ k ↦{c} v' -∗ False;
+    OwnLocalKey_timeless k v :> Timeless (k ↦ₜ v);
+    OwnLocalKey_exclusive k v v' :
+      k ↦ₜ v ⊢ k ↦ₜ v' -∗ False;
 
     (** Laws *)
     ConnectionState_relation E k r ms we :
@@ -65,9 +61,10 @@ Section Resources.
     ⌜k ∈ dom ms →
     ∀ we', ms !! k = Some (Some we') → we' ≤ₜ we ⌝;
 
-   OwnMemKey_OwnLocalKey_coh k we vo c E :
+   OwnMemKey_OwnLocalKey_coh k we c E :
       GlobalInv ⊢
-      k ↦ₖ Some we -∗ k ↦{c} vo ={E}=∗ ⌜is_Some vo⌝;
+      k ↦ₖ Some we -∗ k ↦ₜ c ={E}=∗
+      ∃ we', ⌜c.(cache_snap) = Some we'⌝ ∗ ⌜we' ≤ₜ we⌝;
 
    ConnectionState_Keys E r ms :
     ↑KVS_InvName ⊆ E ->
@@ -81,5 +78,5 @@ Section Resources.
 End Resources.
 (* Arguments SI_resources _ _ : clear implicits. *)
 
-Notation "k ↦ₖ eo" := (OwnMemKey k eo) (at level 20).
-Notation "k ↦{ c } vo" := (OwnLocalKey k c vo) (at level 20).
+Notation "k ↦ₖ e" := (OwnMemKey k e) (at level 20).
+Notation "k ↦ₜ c" := (OwnLocalKey k c) (at level 20).
