aneris/examples/snapshot_isolation/specs/specs_variants/specs_local_pointers.v
@@ -1,0 +1,199 @@
+From iris.algebra Require Import auth gmap excl excl_auth.
+From aneris.algebra Require Import monotone.
+From aneris.aneris_lang Require Import network resources proofmode.
+From aneris.aneris_lang.lib Require Import
+     list_proof inject lock_proof.
+From aneris.aneris_lang.lib.serialization
+     Require Import serialization_proof.
+From aneris.aneris_lang.program_logic Require Import lightweight_atomic.
+From aneris.examples.snapshot_isolation
+     Require Import snapshot_isolation_code_api.
+From aneris.examples.snapshot_isolation.specs
+     Require Import user_params time.
+From aneris.examples.snapshot_isolation.specs.specs_variants
+     Require Import events_local_pointers resources_local_pointers.
+
+Definition cache_commit `{!KVS_time}  c k t : option write_event :=
+    match c.(cache_newv) with
+      | None => c.(cache_snap)
+      | Some v => Some {| we_key := k;  we_val := v; we_time := t; |}
+    end.
+
+Definition max_timestamp `{!KVS_time} t (m : gmap Key (option write_event)) : Prop :=
+    ∀ k (e : write_event), m !! k = Some (Some e) → TM_lt e.(we_time) t.
+
+Definition can_commit `{!KVS_time}
+    (m : gmap Key (option write_event))
+    (mc : gmap Key cache_event) : Prop :=
+    ∀ (k : Key) (ce : cache_event),
+       k ∈ dom m → (mc !! k) = Some ce → is_Some (ce.(cache_newv)) →
+       m !! k = Some ce.(cache_snap).
+
+Definition cache_updv `{!KVS_time} (c : cache_event) (v : val) : cache_event :=
+  {|cache_snap := c.(cache_snap); cache_newv := Some v |}.
+
+Definition cache_getv `{!KVS_time} (c : cache_event) : option val :=
+  match c.(cache_newv) with
+  | Some v => Some v
+  | None =>
+      match c.(cache_snap) with
+      | Some we => Some we.(we_val)
+      | None => None
+      end
+  end.
+
+Definition cache_make `{!KVS_time} (we : option write_event) : cache_event :=
+  {|cache_snap := we; cache_newv := None |}.
+
+Definition kvs_snap_coh `{!KVS_time}
+  (ms m : gmap Key (option write_event)) : Prop :=
+  dom m = dom ms ∧
+    ∀ k we, k ∈ dom ms →
+       ms !! k = Some (Some we) →
+      ∃ we', m !! k = Some (Some we') ∧ we ≤ₜ we'.
+
+Definition snap_cache_coh `{!KVS_time}
+  (ms : gmap Key (option write_event)) (mc : gmap Key cache_event) : Prop :=
+  dom ms = dom mc ∧
+    ∀ k (wo : option write_event), k ∈ dom ms →
+       ms !! k = Some wo →
+      ∃ c, mc !! k = Some c ∧ c.(cache_snap) = wo.
+
+
+(** Specifications for read and write operations.  *)
+Section Specification.
+  Context `{!anerisG Mdl Σ, !User_params, !KVS_time,
+            !KVS_snapshot_isolation_api, !SI_resources Mdl Σ}.
+
+
+  Definition write_spec : iProp Σ :=
+    ∀ (cstate : val) (sa : socket_address)
+      (c : cache_event)
+      (k : Key) (v : SerializableVal) E,
+    ⌜k ∈ KVS_keys⌝ -∗
+    {{{ k ↦ₜ c }}}
+      SI_write cstate #k v @[ip_of_address sa] E
+    {{{ RET #(); k ↦ₜ cache_updv c v }}}.
+
+  Definition read_spec : iProp Σ :=
+    ∀ (cstate : val) (sa : socket_address)
+      (k : Key) (c : cache_event) E,
+    {{{ k ↦ₜ c }}}
+      SI_read cstate #k @[ip_of_address sa] E
+    {{{ vo, RET vo; ⌜vo = $(cache_getv c)⌝ ∗ k ↦ₜ c }}}.
+
+  Definition start_spec : iProp Σ :=
+    ∀ (cstate : val) (sa : socket_address)
+       (E : coPset),
+    ⌜↑KVS_InvName ⊆ E⌝ -∗
+    <<< ∀∀ (m : gmap Key (option write_event)),
+       ConnectionState cstate CanStart ∗
+       [∗ map] k ↦ eo ∈ m, k ↦ₖ eo >>>
+      SI_start cstate @[ip_of_address sa] E
+    <<<▷ RET #();
+       ConnectionState cstate (Active m) ∗
+       ([∗ map] k ↦ eo ∈ m, k ↦ₖ eo) ∗
+       ([∗ map] k ↦ eo ∈ m, k ↦ₜ cache_make eo) >>>.
+
+  Definition commit_spec : iProp Σ :=
+   ∀ (cstate : val) (sa : socket_address)
+     (E : coPset),
+    ⌜↑KVS_InvName ⊆ E⌝ -∗
+    <<< ∀∀ (m ms: gmap Key (option write_event))
+           (mc : gmap Key cache_event),
+        ConnectionState cstate (Active ms) ∗
+        ⌜snap_cache_coh ms mc⌝ ∗
+        ([∗ map] k ↦ eo ∈ m, k ↦ₖ eo) ∗
+        ([∗ map] k ↦ c ∈ mc, k ↦ₜ c) >>>
+      SI_commit cstate @[ip_of_address sa] E
+    <<<▷∃∃ b, RET #b;
+        ConnectionState cstate CanStart ∗
+         ⌜kvs_snap_coh ms m⌝ ∗
+        (** Transaction has been commited. *)
+        (⌜b = true⌝ ∗ ⌜can_commit m mc⌝ ∗
+          ∃ (t: Time), ⌜max_timestamp t m⌝ ∗
+            ([∗ map] k↦c ∈ mc,  k ↦ₖ cache_commit c k t)) ∨
+        (** Transaction has been aborted. *)
+         (⌜b = false⌝ ∗ ⌜¬ can_commit m mc⌝ ∗
+           [∗ map] k ↦ eo ∈ m, k ↦ₖ eo) >>>.
+
+Definition run_spec : iProp Σ :=
+    ∀ (cstate : val) (tbody : val)
+      (sa : socket_address) (E : coPset)
+      (P :  gmap Key (option write_event) → iProp Σ)
+      (Q :  gmap Key (option write_event) → gmap Key cache_event → iProp Σ),
+    ⌜↑KVS_InvName ⊆ E⌝ -∗
+      (∀ (m0 : gmap Key (option write_event)),
+         {{{ ([∗ map] k ↦ wo ∈ m0, k ↦ₜ cache_make wo) ∗ P m0 }}}
+           tbody cstate #() @[ip_of_address sa] E
+         {{{ RET #();
+             ∃ (mc : gmap Key cache_event),
+               ⌜dom m0 = dom mc⌝ ∗ ([∗ map] k ↦ c ∈ mc, k ↦ₜ c) ∗ Q m0 mc }}})
+    →
+    <<< ∀∀ m0, ConnectionState cstate CanStart ∗
+               P m0 ∗
+               [∗ map] k ↦ eo ∈ m0, k ↦ₖ eo >>>
+           SI_run cstate tbody @[ip_of_address sa] E
+    <<<▷∃∃ m1 mc b, RET #b;
+               ConnectionState cstate CanStart ∗
+               ⌜kvs_snap_coh m0 m1⌝ ∗
+               (** Transaction has been commited. *)
+               (⌜b = true⌝ ∗ ⌜can_commit m1 mc⌝ ∗
+                ∃ (t: Time), ⌜max_timestamp t m1⌝ ∗
+                  ([∗ map] k↦c ∈ mc,  k ↦ₖ cache_commit c k t) ∗ Q m0 mc) ∨
+               (** Transaction has been aborted. *)
+               (⌜b = false⌝ ∗ ⌜¬ can_commit m1 mc⌝ ∗
+                [∗ map] k ↦ eo ∈ m1, k ↦ₖ eo) >>>.
+
+  Definition init_client_proxy_spec : iProp Σ :=
+    ∀ (sa : socket_address),
+    {{{ unallocated {[sa]} ∗
+        KVS_address ⤇ KVS_si ∗
+        sa ⤳ (∅, ∅) ∗
+        free_ports (ip_of_address sa) {[port_of_address sa]} }}}
+      SI_init_client_proxy (s_serializer KVS_serialization)
+                  #sa #KVS_address @[ip_of_address sa]
+    {{{ cstate, RET cstate; ConnectionState cstate CanStart }}}.
+
+Definition init_kvs_spec : iProp Σ :=
+  {{{ KVS_address ⤇ KVS_si ∗
+        KVS_address ⤳ (∅,∅) ∗
+        free_ports (ip_of_address KVS_address)
+                   {[port_of_address KVS_address]} }}}
+      SI_init_server (s_serializer KVS_serialization)
+        #KVS_address
+        @[(ip_of_address KVS_address)]
+    {{{ RET #(); True }}}.
+
+End Specification.
+
+
+Class KVSG  Σ :=
+  {
+    KVS_lockG :> lockG Σ;
+    (* TODO ... : ... ; *)
+  }.
+
+Definition KVSΣ : gFunctors :=
+  #[ (* TODO ... ; *) lockΣ].
+
+Instance subG_DBΣ {Σ} : subG KVSΣ Σ → KVSG Σ.
+Proof. econstructor; solve_inG. Qed.
+
+Section SI_Module.
+  Context `{!anerisG Mdl Σ, !KVS_time}.
+
+  Class SI_init `{!User_params, !KVS_snapshot_isolation_api} := {
+     SI_init_module E :
+        True ⊢ |={E}=> ∃ (SIRes : SI_resources Mdl Σ),
+       GlobalInv ∗
+       ([∗ set] k ∈ KVS_keys, k ↦ₖ None) ∗
+       init_kvs_spec ∗
+       init_client_proxy_spec ∗
+       read_spec ∗
+       write_spec ∗
+       start_spec ∗
+       commit_spec ∗
+       run_spec }.
+
+End SI_Module.
